piling it on

theories/History.v
@@ -4,61 +4,223 @@ From LambdaST Require Import
   Prefix
   Types.
 
-(* Definition B.32 *)
-Inductive stlc_type : Set :=
-  | STLCUnit
-  | STLCProd (lhs rhs : stlc_type)
-  | STLCSumT (lhs rhs : stlc_type)
-  | STLCList (t : stlc_type)
+Inductive histval : Set :=
+  | HVUnit
+  | HVPair : histval -> histval -> histval
+  | HVInl : histval -> histval
+  | HVInr : histval -> histval
+  | HVNil : histval
+  | HVCons : histval -> histval -> histval
+.
+
+Inductive histty : Set :=
+  | HTUnit
+  | HTProd (lhs rhs : histty)
+  | HTSum (lhs rhs : histty)
+  | HTList (t : histty)
   .
-Hint Constructors stlc_type : core.
+Hint Constructors histty : core.
 
-(* Definition B.31 *)
-Definition hist_ctx := string -> option stlc_type.
-Hint Unfold hist_ctx : core.
+Inductive HistValTyped : histval -> histty -> Prop :=
+| HVTUnit : HistValTyped HVUnit HTUnit
+| HVTPair : forall v1 v2 t1 t2,
+    HistValTyped v1 t1 ->
+    HistValTyped v2 t2 ->
+    HistValTyped (HVPair v1 v2) (HTProd t1 t2)
+| HVTInl : forall v t1 t2,
+    HistValTyped v t1 ->
+    HistValTyped (HVInl v) (HTSum t1 t2)
+| HVTInr : forall v t1 t2,
+    HistValTyped v t2 ->
+    HistValTyped (HVInr v) (HTSum t1 t2)
+| HVTNil : forall t, HistValTyped HVNil (HTList t)
+| HVTCons : forall t v1 v2,
+    HistValTyped v1 t ->
+    HistValTyped v2 (HTList t) ->
+    HistValTyped (HVCons v1 v2) (HTList t)
+.
 
-(* TODO: propose using user-defined types like Coq's `Inductive` EVENTUALLY for e.g. here,
- * where type-level recursion corresponds to streamification (exactly how we use a list below),
- * since it would make these weird cases go away *)
+Inductive HistValAllTyped : list histval -> list histty -> Prop :=
+| HVATnil : HistValAllTyped nil nil
+| HVATcons : forall v vs t ts, HistValTyped v t -> HistValAllTyped vs ts -> HistValAllTyped (cons v vs) (cons t ts)
+.
+
+
 Fixpoint flatten_type t :=
   match t with
   | TyOne
-  | TyEps (* why not a void type? *) =>
-      STLCUnit
+  | TyEps => HTUnit
   | TyDot lhs rhs
   | TyPar lhs rhs =>
-      STLCProd (flatten_type lhs) (flatten_type rhs)
+      HTProd (flatten_type lhs) (flatten_type rhs)
   | TySum lhs rhs =>
-      STLCSumT (flatten_type lhs) (flatten_type rhs)
+      HTSum (flatten_type lhs) (flatten_type rhs)
   | TyStar t =>
-      STLCList (flatten_type t)
+      HTList (flatten_type t)
   end.
 
-Fixpoint flatten_ctx (c : context) : hist_ctx :=
-  match c with
-  | CtxEmpty =>
-      fun _ => None
-  | CtxHasTy x t =>
-      fun z => if eqb x z then Some (flatten_type t) else None
-  | CtxComma lhs rhs
-  | CtxSemic lhs rhs =>
-      let lhs' := flatten_ctx lhs in
-      let rhs' := flatten_ctx rhs in
-      fun z => match rhs' z with None => lhs' z | Some t => Some t end
-      (* NOTE: right precedence *)
+Definition histctx := list histty.
+Hint Unfold histctx : core.
+
+Inductive PrefixFlatten : prefix -> histval -> Prop :=
+| PLEps : PrefixFlatten PfxEpsEmp HVUnit
+| PLOne : PrefixFlatten PfxOneFull HVUnit
+| PLParPair : forall p1 p2 v1 v2,
+    PrefixFlatten p1 v1 ->
+    PrefixFlatten p2 v2 ->
+    PrefixFlatten (PfxParPair p1 p2) (HVPair v1 v2)
+| PLCatBoth : forall p1 p2 v1 v2,
+    PrefixFlatten p1 v1 ->
+    PrefixFlatten p2 v2 ->
+    PrefixFlatten (PfxCatBoth p1 p2) (HVPair v1 v2)
+| PLInl : forall p v,
+    PrefixFlatten p v ->
+    PrefixFlatten (PfxSumInl p) (HVInl v)
+| PLInr : forall p v,
+    PrefixFlatten p v ->
+    PrefixFlatten (PfxSumInr p) (HVInr v)
+| PLDone : PrefixFlatten PfxStarDone HVNil
+| PLCons : forall p p' v v',
+    PrefixFlatten p v ->
+    PrefixFlatten p v' ->
+    PrefixFlatten (PfxStarRest p p') (HVCons v v')
+.
+
+(* TODO: will *)
+Theorem prefix_flatten_det : forall p v v',
+  PrefixFlatten p v ->
+  PrefixFlatten p v' ->
+  v = v'.
+Proof.
+Admitted.
+
+(* TODO: will *)
+Theorem maximal_prefix_flatten : forall p s,
+  PrefixTyped p s ->
+  MaximalPrefix p ->
+  exists v, PrefixFlatten p v /\ HistValTyped v (flatten_type s).
+Proof.
+Admitted.
+
+Inductive HistValLift : type -> histval -> prefix -> Prop :=
+| PFEps : HistValLift eps HVUnit PfxEpsEmp 
+| PFOne : HistValLift TyOne HVUnit PfxOneFull 
+| PFParPair : forall s t p1 p2 v1 v2,
+    HistValLift s v1 p1 ->
+    HistValLift t v2 p2 ->
+    HistValLift (TyPar s t) (HVPair v1 v2) (PfxParPair p1 p2)
+| PFCatBoth : forall s t p1 p2 v1 v2,
+    HistValLift s v1 p1 ->
+    HistValLift t v2 p2 ->
+    HistValLift (TyDot s t) (HVPair v1 v2) (PfxCatBoth p1 p2)
+| PFInl : forall s t p v,
+    HistValLift s v p -> 
+    HistValLift (TySum s t) (HVInl v) (PfxSumInl p)
+| PFInr : forall s t p v,
+    HistValLift t v p ->
+    HistValLift (TySum s t) (HVInr v) (PfxSumInr p)
+| PFDone : forall s, HistValLift (TyStar s) HVNil PfxStarDone 
+| PFCons : forall s p p' v v',
+    HistValLift s v p ->
+    HistValLift (TyStar s) v' p ->
+    HistValLift (TyStar s) (HVCons v v') (PfxStarRest p p')
+.
+
+(* TODO: will *)
+Theorem histval_lift_det : forall s v p p',
+  HistValLift s v p ->
+  HistValLift s v p' ->
+  p = p'.
+Proof.
+Admitted.
+
+(* TODO: will *)
+Theorem histval_lift_fun : forall s v,
+  HistValTyped v (flatten_type s) ->
+  exists p, HistValLift s v p /\ MaximalPrefix p /\ PrefixTyped p s.
+Proof.
+Admitted.
+
+Definition histtm : Set.
+Admitted.
+
+
+Definition histargs := list histtm.
+
+Definition HistTyped : histctx -> histtm -> histty -> Prop.
+Admitted.
+
+Definition HistStep : histtm -> histval -> Prop.
+Admitted.
+
+(* don't prove, opaque. *)
+Theorem HistStep_sound : forall hp t v,
+  HistTyped nil hp t ->
+  HistStep hp v ->
+  HistValTyped v t.
+Proof.
+Admitted.
+
+Inductive HistArgsTyped : histctx -> histargs -> histctx -> Prop :=
+| HATnil : forall o, HistArgsTyped o nil nil
+| HATcons : forall e es t o o',
+    HistTyped o e t ->
+    HistArgsTyped o es o' ->
+    HistArgsTyped o (cons e es) (cons t o')
+.
+
+Inductive HistArgsStep : histargs -> list histval -> Prop :=
+| HASnil : HistArgsStep nil nil
+| HAScons : forall e es v vs, HistStep e v -> HistArgsStep es vs -> HistArgsStep (cons e es) (cons v vs)
+.
+
+(* TODO: will *)
+Theorem HistArgsStep_sound : forall args ts vs,
+  HistArgsTyped nil args ts ->
+  HistArgsStep args vs ->
+  HistValAllTyped vs ts.
+Proof.
+Admitted.
+
+Definition histval_subst_hist (v : histval) (e : histtm) : histtm.
+Admitted.
+
+Fixpoint histval_subst_all_hist (vs : list histval) (e : histtm) : histtm :=
+  match vs with
+    nil => e
+  | cons v vs' => histval_subst_all_hist vs' (histval_subst_hist v e)
   end.
 
-(* TODO: or should this be a `Fixpoint`? *)
-Inductive ToPrefix : type (* lambda-st type! *) -> stlc_type (* term? value? *) -> prefix -> Prop :=
-  .
-Hint Constructors ToPrefix : core.
+Fixpoint histval_subst_all_histargs (vs : list histval) (e : histargs) : histargs :=
+  match e with
+    nil => nil
+  | cons e es => cons (histval_subst_all_hist vs e) (histval_subst_all_histargs vs es)
+  end.
 
-(* TODO: Definition B.33 *)
+Theorem histval_subst_hist_thm : forall t ts e t' v,
+  HistTyped (cons t ts) e t' ->
+  HistValTyped v t ->
+  HistTyped ts (histval_subst_hist v e) t'.
+Proof.
+Admitted.
 
-(* TODO:will
-Assume a set `histtm`
+(* TODO: will *)
+Theorem histval_subst_all_hist_thm : forall ts e t' vs,
+  HistTyped ts e t' ->
+  HistValAllTyped vs ts ->
+  HistTyped nil (histval_subst_all_hist vs e) t'.
+Proof.
+Admitted.
 
-Assume a prop-valued typing judgmetn for them, and a big-step semantics
+(* TODO: will *)
+Theorem histval_subst_all_histargs_thm : forall ts es ts' vs,
+  HistArgsTyped ts es ts' ->
+  HistValAllTyped vs ts ->
+  HistArgsTyped nil (histval_subst_all_histargs vs es) ts'.
+Proof.
+Admitted.
 
-Assume type soundness
-*)
+
+
+
+
