theories/Typing.v
@@ -17,32 +17,33 @@ From LambdaST Require Import
   Derivative
   Environment
   RecSig
+  History
   Types.
 
 (* TODO:will pull in the rest of the rules (nil, cons, star-case)
    
   if done wiht that, wait (requires histctx)
 *)
-Inductive Typed : context -> recsig -> term -> type -> inertness -> Prop :=
-  | TParR : forall G e1 e2 s t i1 i2 i3 rs,
-      Typed G rs e1 s i1 ->
-      Typed G rs e2 t i2 ->
+Inductive Typed : histctx -> context -> recsig -> term -> type -> inertness -> Prop :=
+  | TParR : forall G e1 e2 s t i1 i2 i3 rs o,
+      Typed o G rs e1 s i1 ->
+      Typed o G rs e2 t i2 ->
       i_ub i1 i2 i3 ->
-      Typed G rs (e1, e2) (TyPar s t) i3
-  | TParL : forall G x y z s t e r Gxsyt Gzst i rs,
+      Typed o G rs (e1, e2) (TyPar s t) i3
+  | TParL : forall G x y z s t e r Gxsyt Gzst i rs o,
       x <> y ->
       ~fv G x ->
       ~fv G y ->
       Fill G (CtxComma (CtxHasTy x s) (CtxHasTy y t)) Gxsyt ->
       Fill G (CtxHasTy z (TyPar s t)) Gzst ->
-      Typed Gxsyt rs e r i ->
-      Typed Gzst rs (TmLetPar x y z e) r i
-  | TCatR : forall G D e1 e2 s t i1 i2 i3 rs,
-      Typed G rs e1 s i1 ->
-      Typed D rs e2 t i2 ->
+      Typed o Gxsyt rs e r i ->
+      Typed o Gzst rs (TmLetPar x y z e) r i
+  | TCatR : forall G D e1 e2 s t i1 i2 i3 rs o,
+      Typed o G rs e1 s i1 ->
+      Typed o D rs e2 t i2 ->
       inert_guard (i1 = Inert /\ ~(Nullable s)) i3 ->
-      Typed (CtxSemic G D) rs (e1; e2) (TyDot s t) i3
-  | TCatL : forall G x y z s t e r Gxsyt Gzst i rs,
+      Typed o (CtxSemic G D) rs (e1; e2) (TyDot s t) i3
+  | TCatL : forall G x y z s t e r Gxsyt Gzst i rs o,
       x <> z -> 
       y <> z -> 
       x <> y ->
@@ -50,29 +51,29 @@ Inductive Typed : context -> recsig -> term -> type -> inertness -> Prop :=
       ~fv G y ->
       Fill G (CtxSemic (CtxHasTy x s) (CtxHasTy y t)) Gxsyt ->
       Fill G (CtxHasTy z (TyDot s t)) Gzst ->
-      Typed Gxsyt rs e r i ->
-      Typed Gzst rs(TmLetCat t x y z e) r i
-  | TEpsR : forall G i rs,
-      Typed G rs TmSink TyEps i
-  | TOneR : forall G rs,
-      Typed G rs TmUnit TyOne Jumpy
-  | TVar : forall G x s Gxs i rs,
+      Typed o Gxsyt rs e r i ->
+      Typed o Gzst rs(TmLetCat t x y z e) r i
+  | TEpsR : forall G i rs o,
+      Typed o G rs TmSink TyEps i
+  | TOneR : forall G rs o,
+      Typed o G rs TmUnit TyOne Jumpy
+  | TVar : forall G x s Gxs i rs o,
       Fill G (CtxHasTy x s) Gxs ->
-      Typed Gxs rs (TmVar x) s i
-  | TLet : forall G D Gxs x e e' s t GD i rs,
+      Typed o Gxs rs (TmVar x) s i
+  | TLet : forall G D Gxs x e e' s t GD i rs o,
       ~fv G x ->
-      Typed D rs e s Inert ->
+      Typed o D rs e s Inert ->
       Fill G (CtxHasTy x s) Gxs ->
       Fill G D GD ->
-      Typed Gxs rs e' t i ->
-      Typed GD rs (TmLet x e e') t i
-  | TInl : forall G e s t i rs,
-      Typed G rs e s i ->
-      Typed G rs (TmInl e) (TySum s t) Jumpy
-  | TInr : forall G e s t i rs,
-      Typed G rs e s i ->
-      Typed G rs (TmInr e) (TySum s t) Jumpy
-  | TPlusCase : forall G x y z s t r Gz Gx Gy Gz' e1 e2 eta i i1 i2 rs,
+      Typed o Gxs rs e' t i ->
+      Typed o GD rs (TmLet x e e') t i
+  | TInl : forall G e s t i rs o,
+      Typed o G rs e s i ->
+      Typed o G rs (TmInl e) (TySum s t) Jumpy
+  | TInr : forall G e s t i rs o,
+      Typed o G rs e s i ->
+      Typed o G rs (TmInr e) (TySum s t) Jumpy
+  | TPlusCase : forall G x y z s t r Gz Gx Gy Gz' e1 e2 eta i i1 i2 rs o,
       ~ fv G x ->
       ~ fv G y ->
       Fill G (CtxHasTy z (TySum s t)) Gz ->
@@ -80,47 +81,52 @@ Inductive Typed : context -> recsig -> term -> type -> inertness -> Prop :=
       Fill G (CtxHasTy y t) Gy ->
       EnvTyped eta Gz ->
       ContextDerivative eta Gz Gz' ->
-      Typed Gx rs e1 r i1 ->
-      Typed Gy rs e2 r i2 ->
+      Typed o Gx rs e1 r i1 ->
+      Typed o Gy rs e2 r i2 ->
       inert_guard (eta z = Some PfxSumEmp) i ->
-      Typed Gz' rs (TmPlusCase eta r z x e1 y e2) r i
-  | TRec : forall G G' s i args,
-      ArgsTyped G' (Rec G s i) args G i ->
-      Typed G' (Rec G s i) (TmRec args) s i
-  | TFix : forall G G' rs args e r i,
+      Typed o Gz' rs (TmPlusCase eta r z x e1 y e2) r i
+  | TRec : forall G G' s i args o o' hpargs,
+      HistArgsTyped o hpargs o' ->
+      ArgsTyped o G' (Rec o' G s i) args G i ->
+      Typed o G' (Rec o' G s i) (TmRec args hpargs) s i
+  | TFix : forall G G' rs args e r i o o' hpargs,
       WFContext G ->
-      ArgsTyped G' rs args G i ->
-      Typed G (Rec G r i) e r i ->
-      Typed G' rs (TmFix args G r e) r i
-  | TmArgsLet : forall G G' args e rs s i,
+      HistArgsTyped o' hpargs o ->
+      ArgsTyped o' G' rs args G i ->
+      Typed o G (Rec o G r i) e r i ->
+      Typed o' G' rs (TmFix args hpargs G r e) r i
+  | TmArgsLet : forall G G' args e rs s i o,
       WFContext G ->
-      ArgsTyped G' rs args G i ->
-      Typed G rs e s i ->
-      Typed G' rs (TmArgsLet args G e)  s i
-  | TSubCtx : forall G G' e s i rs,
+      ArgsTyped o G' rs args G i ->
+      Typed o G rs e s i ->
+      Typed o G' rs (TmArgsLet args G e)  s i
+  | TmHistPgm : forall G rs hp s o,
+      HistTyped o hp (flatten_type s) ->
+      Typed o G rs (TmHistPgm hp s) s Jumpy
+  | TSubCtx : forall G G' e s i rs o,
       Subcontext G G' ->
-      Typed G' rs e s i ->
-      Typed G rs e s i
+      Typed o G' rs e s i ->
+      Typed o G rs e s i
       
-with ArgsTyped : context -> recsig -> argsterm -> context -> inertness -> Prop :=
-  | T_ATmEmpty : forall g rs i, ArgsTyped g rs ATmEmpty CtxEmpty i
-  | T_ATmSng : forall g rs e s x i,
-      Typed g rs e s i ->
-      ArgsTyped g rs (ATmSng e) (CtxHasTy x s) i
-  | T_ATmComma : forall g g1 g2 e1 e2 rs i1 i2 i3,
-      ArgsTyped g rs e1 g1 i1 ->
-      ArgsTyped g rs e2 g2 i2 ->
+with ArgsTyped : histctx -> context -> recsig -> argsterm -> context -> inertness -> Prop :=
+  | T_ATmEmpty : forall g rs i o, ArgsTyped o g rs ATmEmpty CtxEmpty i
+  | T_ATmSng : forall g rs e s x i o,
+      Typed o g rs e s i ->
+      ArgsTyped o g rs (ATmSng e) (CtxHasTy x s) i
+  | T_ATmComma : forall g g1 g2 e1 e2 rs i1 i2 i3 o,
+      ArgsTyped o g rs e1 g1 i1 ->
+      ArgsTyped o g rs e2 g2 i2 ->
       i_ub i1 i2 i3 ->
-      ArgsTyped g rs (ATmComma e1 e2) (CtxComma g1 g2) i3
-  | T_ATmSemic1 : forall g1 g2 g1' g2' e1 e2 rs i1 i2 i3,
-      ArgsTyped g1 rs e1 g1' i1 ->
-      ArgsTyped g2 rs e2 g2' i2 ->
+      ArgsTyped o g rs (ATmComma e1 e2) (CtxComma g1 g2) i3
+  | T_ATmSemic1 : forall g1 g2 g1' g2' e1 e2 rs i1 i2 i3 o,
+      ArgsTyped o g1 rs e1 g1' i1 ->
+      ArgsTyped o g2 rs e2 g2' i2 ->
       inert_guard (i1 = Inert /\ ~(NullableCtx g1')) i3 ->
-      ArgsTyped (CtxSemic g1 g2) rs (ATmSemic1 e1 e2) (CtxSemic g1' g2') i3
-  | T_ATmSemic2 : forall g1 g2 g1' g2' e2 rs i,
+      ArgsTyped o (CtxSemic g1 g2) rs (ATmSemic1 e1 e2) (CtxSemic g1' g2') i3
+  | T_ATmSemic2 : forall g1 g2 g1' g2' e2 rs i o,
       NullableCtx g1' ->
-      ArgsTyped g2 rs e2 g2' i ->
-      ArgsTyped (CtxSemic g1 g2) rs (ATmSemic2 e2) (CtxSemic g1' g2') i
+      ArgsTyped o g2 rs e2 g2' i ->
+      ArgsTyped o (CtxSemic g1 g2) rs (ATmSemic2 e2) (CtxSemic g1' g2') i
 .
 
 Scheme Typed_ind' := Induction for Typed Sort Prop
@@ -133,18 +139,18 @@ Hint Constructors ArgsTyped : core.
 Check Typed_mutual.
 
 Theorem typing_fix_subst_mut :
-  (forall (g' : context) (rs: recsig) e' t i', Typed g' rs e' t i' -> 
-    forall g e s i,
-      Typed g (Rec g s i) e s i ->
+  (forall o' (g' : context) (rs: recsig) e' t i', Typed o' g' rs e' t i' -> 
+    forall o g e s i,
+      Typed o g (Rec o g s i) e s i ->
       WFContext g ->
-      rs = Rec g s i ->
-      Typed g' NoRec (fix_subst g s e e') t i') /\
-  (forall g' (rs: recsig) args g'' i', ArgsTyped g' rs args g'' i' ->
-    forall g e s i,
-      Typed g (Rec g s i) e s i ->
+      rs = Rec o g s i ->
+      Typed o' g' NoRec (fix_subst g s e e') t i') /\
+  (forall o' g' (rs: recsig) args g'' i', ArgsTyped o' g' rs args g'' i' ->
+    forall o g e s i,
+      Typed o g (Rec o g s i) e s i ->
       WFContext g ->
-      rs = Rec g s i ->
-      ArgsTyped g' NoRec (fix_subst_args g s e args) g'' i').
+      rs = Rec o g s i ->
+      ArgsTyped o' g' NoRec (fix_subst_args g s e args) g'' i').
 intros.
   apply Typed_mutual; cbn; intros.
   - econstructor. { eapply H; eauto. } { eapply H0; eauto. } hauto l: on.
@@ -163,17 +169,18 @@ intros.
   - hauto l: on.
   - hauto l: on.
   - hauto l: on.
+  - hauto l: on.
   - sauto lq: on.
   - intros. econstructor. { eapply H; eauto. } { eapply H0; eauto. } sfirstorder.
   - intros. econstructor. { eapply H; eauto. } { eapply H0; eauto. } sfirstorder.
   - hauto l: on.
 Qed.
 
-Theorem typing_fix_subst : forall g g' e e' s t i i',
+Theorem typing_fix_subst : forall g g' e e' s t i i' o o',
   WFContext g ->
-  Typed g (Rec g s i) e s i ->
-  Typed g' (Rec g s i) e' t i' -> 
-  Typed g' NoRec (fix_subst g s e e') t i'.
+  Typed o g (Rec o g s i) e s i ->
+  Typed o' g' (Rec o g s i) e' t i' -> 
+  Typed o' g' NoRec (fix_subst g s e e') t i'.
 Proof.
 sfirstorder use:typing_fix_subst_mut.
 Qed.
@@ -243,18 +250,18 @@ Hint Resolve fv_hole_minus : core.
 (* (P : ∀ (c : context) (t : term) (t0 : type) (i : inertness),
        Typed c t t0 i → Prop) *)
 
-Definition P_typing_fv (g : context) (rs : recsig) (e : term) (s : type) (i : inertness) :=
+Definition P_typing_fv (o : histctx) (g : context) (rs : recsig) (e : term) (s : type) (i : inertness) :=
   forall x, fv e x -> fv g x.
-Arguments P_typing_fv g rs e s i/.
+Arguments P_typing_fv o g rs e s i/.
 
-Definition P_argstyping_fv (g : context) (rs : recsig) (args : argsterm) (g' : context) (i : inertness) :=
+Definition P_argstyping_fv (o : histctx) (g : context) (rs : recsig) (args : argsterm) (g' : context) (i : inertness) :=
   forall x, fv args x -> fv g x.
-Arguments P_argstyping_fv g rs args g' i/.
+Arguments P_argstyping_fv o g rs args g' i/.
 
 (* TODO: will: priority *)
 Theorem typing_fv' :
-  (forall g rs e s i, Typed g rs e s i -> P_typing_fv g rs e s i) /\
-  (forall g rs args g' i, ArgsTyped g rs args g' i -> P_argstyping_fv g rs args g' i).
+  (forall o g rs e s i, Typed o g rs e s i -> P_typing_fv o g rs e s i) /\
+  (forall o g rs args g' i, ArgsTyped o g rs args g' i -> P_argstyping_fv o g rs args g' i).
 Proof.
   apply Typed_mutual; cbn in *; intros.
  - sfirstorder.
@@ -279,7 +286,9 @@ Proof.
  - sfirstorder.
  - sfirstorder.
  - sfirstorder.
+ - sfirstorder.
  - sfirstorder use:subcontext_fv_subset.
+ - sfirstorder.
  - sfirstorder.
  - sfirstorder.
  - sfirstorder.
@@ -331,15 +340,15 @@ Proof.
   induction H; hauto l:on use:typing_fv'.
 Qed. *)
 
-Theorem typing_fv : forall G e s i rs,
-  Typed G rs e s i ->
+Theorem typing_fv : forall G e s i rs o,
+  Typed o G rs e s i ->
   Subset (fv e) (fv G).
 Proof.
 best use:typing_fv'.
 Qed.
 
-Theorem typing_fv_args : forall G G' e i rs,
-  ArgsTyped G rs e G' i ->
+Theorem typing_fv_args : forall G G' e i rs o,
+  ArgsTyped o G rs e G' i ->
   Subset (fv e) (fv G).
 Proof.
 best use:typing_fv'.
@@ -347,17 +356,18 @@ Qed.
 
 Hint Resolve typing_fv : core.
 
-Theorem sink_tm_typing : forall g p s s' rs,
+Theorem sink_tm_typing : forall g p s s' rs o,
   PrefixTyped p s ->
   MaximalPrefix p ->
   Derivative p s s' ->
-  Typed g rs (sink_tm p) s' Inert.
+  Typed o g rs (sink_tm p) s' Inert.
 Proof.
-intros g p s s' rs Ht Hm.
+intros g p s s' rs o Ht Hm.
 generalize dependent s'.
 generalize dependent g.
 generalize dependent rs.
-dependent induction Ht; sinvert Hm; cbn; intros rs g s' Hd.
+generalize dependent o.
+dependent induction Ht; sinvert Hm; cbn; intros o rs g s' Hd.
 - best.
 - best.
 - sinvert Hd. econstructor; sfirstorder.
@@ -370,15 +380,15 @@ Qed.
 
 
 (* Todo: will: PRIORITY. *)
-Theorem typing_subst : forall h e x y s t i gx gy rs,
-  Typed gx rs e t i ->
+Theorem typing_subst : forall h e x y s t i gx gy rs o,
+  Typed o gx rs e t i ->
   WFContext gx ->
   ~ fv h y ->
   Fill h (CtxHasTy x s) gx ->
   Fill h (CtxHasTy y s) gy ->
-  Typed gy rs (subst_var e y x) t i.
+  Typed o gy rs (subst_var e y x) t i.
 Proof.
-  intros h e x y s t i gx gy rs Ht Hw Hn Hx Hy.
+  intros h e x y s t i gx gy rs o Ht Hw Hn Hx Hy.
   generalize dependent gy.
   generalize dependent s.
   generalize dependent y.
@@ -402,3 +412,31 @@ Proof.
   - admit.
   - admit.
 Admitted.
+
+Theorem typing_histval_subst_all : 
+  (forall o g rs e s i, Typed o g rs e s i -> forall vs, HistValAllTyped vs o -> Typed nil g rs (histval_subst_all vs e) s i) /\ 
+  (forall o g rs args g' i, ArgsTyped o g rs args g' i -> forall vs, HistValAllTyped vs o -> ArgsTyped nil g rs (histval_subst_all_args vs args) g' i).
+Proof.
+  apply Typed_mutual; intros.
+  - cbn. econstructor. eauto. eauto. sfirstorder.
+  - sfirstorder.
+  - sfirstorder.
+  - sfirstorder.
+  - sfirstorder.
+  - sfirstorder.
+  - sfirstorder.
+  - sfirstorder.
+  - sfirstorder.
+  - sfirstorder.
+  - sfirstorder.
+  - sfirstorder use: histval_subst_all_histargs_thm.
+  - hauto l:on use: histval_subst_all_histargs_thm.
+  - sfirstorder.
+  - sfirstorder use:histval_subst_all_hist_thm.
+  - sfirstorder.
+  - sfirstorder.
+  - sfirstorder.
+  - cbn. econstructor; sfirstorder.
+  - sfirstorder.
+  - sfirstorder.
+Qed.
